commit-2

EasyTeach/Cyclic_group_prime.ec
@@ -5,12 +5,17 @@ require import Distr.
 
 type group.
 const g:group. (* the generator *)
+const id:group.
+
+
 
 op ( ** ): group -> group -> group.   (* multiplication of group elements *)
 op ( ^ ): group -> gf_q -> group.    (* exponentiation *)
 op log:group -> gf_q.                (* discrete logarithm *)
 
 op (//) (a b:group): group = g^(log a - log b).
+
+op inv: group -> group.
 
 axiom group_pow_add: forall (x y:gf_q),
   g ^ x ** g ^ y = g ^ (x + y).
@@ -24,9 +29,25 @@ axiom group_log_pow: forall (a:group),
 axiom group_pow_log: forall (x:gf_q),
   log (g ^ x) = x.
 
+(*axiom inverse_group: forall (x:group),
+  (exists (x_inv : group), true),
+  x**x_inv = x_inv**x = id.*)
+
+axiom mul_id : forall(x: group),
+  x**id = id**x /\ x**id = x.
+
+axiom group_order: exists (q:gf_q),
+(g^q) = id. (* fix me -- this doesn't give the order of g *)
+
+(*axiom exp_ele: forall(x:group),
+ x = g^r.
+
+*)
 
 theory Dgroup.
-  op dgroup: group distr.
+op dgroup: group distr.
+
+op dgf_q: gf_q distr.
 
   axiom supp_def: forall (s:group),
     support dgroup s.
